MPPA: Conditional and unconditional branches
Conditional branches are implemented the naïve way by evaluating the
comparison's result into register R63 (this choice is arbitrary, but
CompCert forces us to fix one register), then branching on this register's
zero/non-zero status. There is room for optimization: integer comparisons
against 0 (or even/odd tests) could be folded into the conditional branch.

mppa/TargetPrinter.ml
@@ -257,8 +257,24 @@ struct
     | FTuge -> "uge"
     | FToge -> "oge"
     | FTult -> "ult"
+    | _ ->
+      (* Conditions used in modeling, but not provided by the hardware. We
+         should never generate these. *)
+      assert false
 
   let fcond oc c = fprintf oc "%s" (fcond_name c)
+
+  let bcond_name = function
+    | BTnez  -> "nez"
+    | BTeqz  -> "eqz"
+    | BTltz  -> "ltz"
+    | BTgez  -> "gez"
+    | BTlez  -> "lez"
+    | BTgtz  -> "gtz"
+    | BTodd  -> "odd"
+    | BTeven -> "even"
+
+  let bcond oc c = fprintf oc "%s" (bcond_name c)
 
     (*
   let condition_name = function
@@ -628,8 +644,14 @@ struct
     (* Branch control unit instructions *)
     | Pcall (symb, _sig) ->
       fprintf oc "	call %a\n	;;\n" symbol symb; 1
+    | Pcb (cond, rs, lbl) ->
+      fprintf oc "	cb.%a %a, %a\n	;;\n" bcond cond gpreg rs print_label lbl; 1
+    | Pcdb (cond, rs, lbl) ->
+      fprintf oc "	cdb.%a %a, %a\n	;;\n" bcond cond pgpreg rs print_label lbl; 1
     | Pget (rd, rs) ->
       fprintf oc "	get %a = %a\n	;;\n" gpreg rd preg rs; 1
+    | Pgoto lbl ->
+      fprintf oc "	goto %a\n	;;\n" print_label lbl; 1
     | Picall (r, _sig) ->
       fprintf oc "	icall %a\n	;;\n" gpreg r; 1
     | Pret ->
@@ -652,8 +674,11 @@ struct
       fprintf oc "	addd %a = %a, %a\n	;;\n" pgpreg rd pgpreg r1 preg_or_imm op2; 1
     | Pcomp (c, rd, r1, op2) ->
       fprintf oc "	comp.%a %a = %a, %a\n	;;\n" icond c gpreg rd gpreg r1 reg_or_imm op2; 1
-    | Pcompdl (c, rd, r1, op2) ->
-      fprintf oc "	compdl.%a %a = %a, %a\n	;;\n" icond c gpreg rd pgpreg r1 preg_or_imm op2; 1
+    | Pcompdl (c, rd, r1, PRIimm n) ->
+      (* The double register argument must be printed as a pasted pair. *)
+      fprintf oc "	compdl.%a %a = %a, %a\n	;;\n" icond c gpreg rd pgpreg_pair r1 coqint n; 1
+    | Pcompdl (c, rd, r1, PRIreg r2) ->
+      fprintf oc "	compdl.%a %a = %a, %a\n	;;\n" icond c gpreg rd pgpreg r1 pgpreg r2; 1
     | Pmake (rd, n) ->
       fprintf oc "	make %a = %a\n	;;\n" gpreg rd coqint n; 1
     | Pmaked (rd, n) ->
